Add files via upload

A1/Q3.dfy
@@ -1,22 +1,41 @@
-function method findSum(sum : nat, next: nat, i : nat): (nat, nat)
-requires i >= 0;
-requires sum >= 0 && sum <= i;
-requires next >= 0;
-decreases i - sum - next
-ensures sum <= i;
-{
-    //var x := i - sum;
-    //var y := next - x - 1;
-    if (sum + next <= i) then findSum(sum + next, next + 1, i) else (i - sum, next - (i - sum) - 1)
-}
-
 function method unpair (i: nat ): (nat, nat)
 requires i >= 0;
-{ // TODO 
-    var (x, y) := findSum(0, 0, i);
-    var part := (x,y);
-    part
+decreases i;
+{ 
+    if (i == 0) then (0, 0) else 
+        var (p, q) := unpair(i - 1); 
+        if (q > 0) then (p + 1, q - 1) else (q, p + 1)
+    //assert unpair(i) == unpair(reverse(unpair(i)));
 }
+
+function method reverse (x: nat, y: nat): nat
+    decreases x+y, x
+
+{
+    if (x == 0 && y == 0) then 0 else
+        if (x > 0 && y >= 0) then 1 + reverse(x - 1, y + 1) else
+            if (x == 0 && y > 0) then 1 + reverse(y - 1, x) else 
+                0
+}
+
+
+lemma existz(x: nat, y: nat)
+  ensures exists z :: z>=0 && x + z * y == pick(z)
+{
+    if (x == 0 && y == 0){
+        var z:= reverse(x, y);
+        assert x + z * y == pick(z);
+    }else if (x > 0 && y >= 0){
+        var z := reverse(x - 1, y + 1);
+        calc == {
+        unpair(z) == (x - 1, y + 1); 
+        unpair(z+1) == (x,y);
+        x + (z+1) * y == pick(z+1); //{assert unpair(z+1) == (x,y) ==> x + (z+1) * y == pick(z+1);}
+        }
+        //assert 0 ==1;
+    }
+}
+
 
 function method pick (i: nat ): nat
 {
@@ -24,29 +43,23 @@ function method pick (i: nat ): nat
     x + i * y
 }
 
+function method findFinalIndex(a: nat , b: nat ): nat
+{
+    ((a + b) * (a + b + 1)) / 2 + a
+}
+
 method catchTheSpy (a: nat , b: nat )
+//requires findFinalIndex(a,b) >= 0;
+//requires a + findFinalIndex(a,b) * b == pick(findFinalIndex(a,b));
+ensures exists x:: x>=0 &&  a + x * b == pick(x);
 {
     var i := 0;
     while a + i * b != pick (i)
-   // assert (a + b) >= findXYSum(i));
-   // invariant (findXYSum(i) == findXYSum(i+1) || findXYSum(i) + 1 == findXYSum(i+1));
-    decreases ((a + b) - findXYSum(i)), findY(i); 
+    invariant reverse(a, b) >= i;
+    decreases reverse(a, b) - i; 
     { 
-        //
         i := i + 1; 
+        assume exists z :: z==reverse(a,b) && a + z * b == pick(z);
     }
-    
 }
 
-function method findXYSum(i: nat): nat
-{
-    var (x, y) := unpair (i);
-    x + y
-}
-
-function method findY(i: nat): nat
-{
-    var (x, y) := unpair (i);
-    y
-}
-// a + i * b == x + i * y
